EffectSSA/Trace/Defs.lean
@@ -1,4 +1,6 @@
 import EffectSSA.Assumptions.MemorySignature
+import EffectSSA.Assumptions.Compat
+import EffectSSA.ITC
 
 import Mathlib.Data.Set.Defs
 import Mathlib.Data.Set.Operations
@@ -13,8 +15,14 @@ This file defines memory events, and traces of such events
 namespace EffectSSA
 variable (τ : Ty) [MemorySignature τ]
 
+open ITC (Clock)
+noncomputable section -- TODO: remove once ITC has been implemented
+-- ^^ The following definitions use `Clock` axioms, and thus are noncomputable
+--    untill we actually implement the Clock module.
+
 /-!
 ## Event Definition
+--------------------------------------------------------------------------------
 -/
 
 inductive Event where
@@ -29,58 +37,84 @@ inductive Event where
   | split
   deriving DecidableEq
 
+/--
+A `ClockedEvent τ c` is a `Event τ` tagged with some clock-value, which is
+statically known to have happened before `c`.
+-/
+structure ClockedEvent (c : Clock) where
+  clock : Clock
+  event : Event τ
+  clock_le : clock ≤ c := by grind
+  deriving DecidableEq
+
+/--
+Two clocked events are compatible when either their clocks are ordered in either
+direction (i.e, the events did not happen concurrently), or the underlying
+events are compatible (i.e., the side-effects commute).
+-/
+instance [Compat (Event τ)] : HCompat (ClockedEvent τ c) (ClockedEvent τ c') where
+  hCompat x y := x.clock # y.clock → x.event ⌣ y.event
+
 /-!
 ## Trace Definition
+--------------------------------------------------------------------------------
 -/
+variable [Compat (Event τ)]
 
-inductive Trace where
-  | seq : List (Event τ) → Trace
-  | ub : Trace
+structure Trace where
+  /-- The current clock for the corresponding thread. -/
+  clock : Clock
+  events : List (ClockedEvent τ clock)
+  /-- Whether UB has been raised. -/
+  isUB : Bool
+  /-- All events in a (non-UB) trace ought to be pairwise compatible. -/
+  compat : ¬isUB → events.Pairwise (· ⌣ ·) := by solve | simp | grind
   deriving DecidableEq
 
 /-!
-### API
+## API
+--------------------------------------------------------------------------------
 -/
 variable {τ}
 
-/-! ## Event API -/
-namespace Event
+/-! ### ClockedEvent API -/
+namespace ClockedEvent
 
-/- An `Event` may be implicitly coerced to a `Trace`. -/
-instance : Coe (Event τ) (Trace τ) where
-  coe e := .seq [e]
+def cast_le (h : c ≤ c' := by grind) (e : ClockedEvent τ c) : ClockedEvent τ c' :=
+  { e with clock_le := by grind [e.clock_le] }
 
-end Event
+end ClockedEvent
 
-/-! ## Trace API -/
+/-! ### Trace API -/
 namespace Trace
 
-/-- A list of `Event`s may be implicitly coerced to a `Trace`. -/
-instance : Coe (List (Event τ)) (Trace τ) where
-  coe := .seq
 
 /-- `∅` is the empty (non-UB) trace, without any events. -/
 instance : EmptyCollection (Trace τ) where
-  emptyCollection := .seq []
+  emptyCollection := { clock := .initial, events := [], isUB := false }
 
 /--
 Add a new event to the front of a trace,
 where adding an event onto a UB trace just yields UB.
 
+The new event will be recorded with the current clock value stored in the trace.
+
 Written as `e :> ev`
 -/
-def cons (e : Event τ) : Trace τ → Trace τ
-  | .seq ev => seq (e :: ev)
-  | .ub => .ub
+def cons (e : Event τ) (es : Trace τ) : Trace τ :=
+  let e := { clock := es.clock, event := e }
+  { es with
+    events := e :: es.events
+    compat := by
+      have (e' : ClockedEvent τ es.clock) : e ⌣ e' := by
+        intro hc
+        have : e.clock = es.clock := rfl
+        have := e'.clock_le
+        grind
+      intro hUB
+      simp [es.compat hUB, this]
+  }
 @[inherit_doc] infixr:67 " :> " => cons
-
-/--
-Append two traces.
--/
-def append : Trace τ → Trace τ → Trace τ
-  | .seq xs, .seq ys => .seq (xs ++ ys)
-  | _, _ => .ub
-instance : Append (Trace τ) where append := append
 
 /--
 A `TraceZipper` points to a specific event in a (non-UB) trace, while also
@@ -107,10 +141,34 @@ structure TraceZipper τ [MemorySignature τ] where
 --   of the trace, but have the wrong chronological implication!
 
 
-def events : Trace τ → Set (TraceZipper τ)
-  | .ub => {}
-  | .seq es => { ⟨es.take i, es[i], es.drop (i + 1)⟩ | (i : Fin es.length)}
-
-
+def eventSet (es : Trace τ) : Set (TraceZipper τ) :=
+  if !es.isUB then
+    let ev := es.events.map (·.event)
+    { ⟨ev.take i, ev[i], ev.drop (i + 1)⟩ | (i : Fin ev.length)}
+  else
+    ∅
 
 end Trace
+
+/-
+## Basic Lemmas
+--------------------------------------------------------------------------------
+
+Lemmas needed to prove invariants for further definitions.
+-/
+
+namespace ClockedEvent
+variable (x : ClockedEvent τ c₁) (y : ClockedEvent τ c₂)
+
+@[simp, grind =] theorem cast_le_compat (h : c₁ ≤ c₁') :
+    x.cast_le h ⌣ y ↔ x ⌣ y := by
+  sorry
+
+@[simp, grind =] theorem compat_cast_le (h : c₂ ≤ c₂') :
+    x ⌣ y.cast_le h ↔ x ⌣ y := by
+  sorry
+
+@[grind =>] theorem compat_of_not_unrel (h : ¬(x.clock # x.clock)) : x ⌣ y := by
+  sorry
+
+end ClockedEvent
