EffectSSA/Assumptions/Compat.lean
@@ -1,0 +1,42 @@
+
+/-!
+# Compatibility Notation Typeclass
+-/
+namespace EffectSSA
+
+/--
+`Compat α` is the typeclass which supports the notation `x ⌣ y`, where `x, y : α`.
+That is, it's a convenience wrapper for `HCompat`.
+
+The precise meaning of this relation is type-dependent, but it generally revolves
+around some notion of commuting side-effects.
+-/
+class Compat (α : Type u) where
+  /-- The compatibility relation: `x ⌣ y` -/
+  compat : α → α → Prop
+
+/--
+`HCompat α β` is the typeclass which supports the notation `x ⌣ y`, where `x : α`
+and `y : β`.
+
+The precise meaning of this relation is type-dependent, but it generally revolves
+around some notion of commuting side-effects.
+-/
+class HCompat (α : Type u) (β : Type v) where
+  /-- The compatibility relation: `x ⌣ y` -/
+  hCompat : α → β → Prop
+
+@[inherit_doc] infixl:60 " ⌣ " => HCompat.hCompat
+
+/-- An instance of `Copmat` implies an instance of `HCompat` -/
+instance [Compat α] : HCompat α α where
+  hCompat := Compat.compat
+
+/--
+An abbreviation for `DecidableRel` of the (heterogeneous) compatibility
+relation on `α` and `β`.
+-/
+abbrev DecidableHCompat (α β) [HCompat α β] := DecidableRel (· ⌣ · : α → β → Prop)
+
+/-- An abbreviation for `DecidableRel` of the compatibility relation on `α`. -/
+abbrev DecidableCompat (α) [Compat α] := DecidableHCompat α α
